Add an outline for lecture 1

lecture1.dfy
@@ -1,10 +1,78 @@
 /* Mathematical assertions */
 lemma SomeAssertions() {
-    assert 2 + 2 == 4;
-    assert 1 < 2;
-    assert -3*-2 == -6;
-    assert 1 + 2*3 == 7;
+  assert 2 + 2 == 4;
+  assert 1 < 2;
+  assert -3*-2 == -6;
+  assert 1 + 2*3 == 7;
 }
 
+/* a function is a mathematical function: it is always deterministic, and is
+  written without mutable variables or data structures */
+
 function abs(x: int): int {
+  /* if is an expression */
+  if x < 0 then -x else x
 }
+
+/* We can prove things about functions using lemmas.
+
+   This lemma has a parameter. When we use the lemma, that parameter is just
+   like a function argument: we'll call AbsLarger on some specific x.
+ */
+lemma AbsLarger(x: int)
+  ensures abs(x) >= x
+{}
+
+/* this property isn't true */
+lemma AbsStrictlyLarger(x: int)
+  ensures abs(x) > x
+{
+  // we can invoke the already-proven lemma like this - but it doesn't actually
+  // help prove the postcondition in this case
+  AbsLarger(x);
+  // Next we could try splitting the proof into two cases, which looks just like
+  // an if statement in imperative code.
+  if x < 0 {
+    // there's no error here! the postcondition actually does hold on this path
+  } else {
+    // But here if we think about it we realize abs(x) == x.
+    assert abs(x) == x;
+  }
+}
+
+lemma AbsNegLarger(x: int)
+  requires x < 0
+  ensures abs(x) > x
+{}
+
+/* Quantifiers */
+
+lemma AbsLargerForAll()
+  ensures forall x: int :: abs(x) >= x
+{
+  // new syntax: forall statement
+  forall x: int
+    ensures abs(x) >= x
+  {
+    // this statement allows us to refer to x when proving a forall, which means
+    // we can call lemmas, do `if` case splits, etc.
+    AbsLarger(x);
+  }
+}
+
+/* This lemma shows, in a roundabout way, that positive numbers have a negative
+ * with the same absolute value. */
+lemma PosHasNeg(x: int)
+  requires x > 0
+  ensures exists y :: y < 0 && abs(y) == x
+{
+  // Dafny needs some help here to find a "witness" for y, which proves the
+  // exists. In this case it's pretty simple to see that the y that exists is
+  // -x.
+  var y := -x;
+  // This assertion nudges Dafny along to use y to prove the postcondition. Not
+  // all of this is necessary but it's good practice.
+  assert y < 0 && abs(y) == x;
+}
+
+/* TODO: assign such that? what would the example be? */
